Implement one-tick Force in env-semantics
The env-based semantics deals with this in a less elegant way
(binding the 'next' value to a dummy variable, instead of lifting
it into an expression using Value).

compiler/backend/thunkLangScript.sml
@@ -6,6 +6,9 @@
    - It has a call-by-value semantics.
    - It extends the pureLang syntax with explicit syntax for delaying and
      forcing computations (“Delay” and “Force”) and “Thunk” values.
+   - Suspended computations can be wrapped in “MkTick” to cause the suspended
+     evaluation to consume one extra clock tick by producing a value wrapped in
+     “DoTick”.
    - This version has an environment-based semantics. See
      [thunkLang_substScript.sml] for a substitution-based version.
  *)
@@ -29,6 +32,7 @@ Datatype:
       | Delay exp                                (* suspend in a Thunk      *)
       | Box exp                                  (* wrap result in a Thunk  *)
       | Force exp                                (* evaluates a Thunk       *)
+      | MkTick exp                               (* creates a delayed Tick  *)
 End
 
 Datatype:
@@ -37,6 +41,7 @@ Datatype:
     | Recclosure ((vname # exp) list) ((vname # v) list) vname
     | Thunk (v + (vname # v) list # exp)
     | Atom lit
+    | DoTick v                                   (* extra clock when forced *)
 End
 
 Definition subst_funs_def[simp]:
@@ -63,6 +68,11 @@ Definition dest_anyClosure_def:
         SOME (Lam s x) => return (s, subst_funs f env, x)
       | _ => fail Type_error
     od
+End
+
+Definition dest_Tick_def[simp]:
+  dest_Tick (DoTick v) = SOME v ∧
+  dest_Tick _ = NONE
 End
 
 Definition dest_Thunk_def[simp]:
@@ -107,7 +117,8 @@ Definition freevars_def:
      set (MAP FST f)) ∧
   freevars (Delay x) = freevars x ∧
   freevars (Box x) = freevars x ∧
-  freevars (Force x) = freevars x
+  freevars (Force x) = freevars x ∧
+  freevars (MkTick x) = freevars x
 Termination
   WF_REL_TAC ‘measure exp_size’
   \\ rw []
@@ -118,6 +129,10 @@ End
 
 Definition closed_def:
   closed e ⇔ freevars e = ∅
+End
+
+Definition dummy_def:
+  dummy = "%dummy%"
 End
 
 Definition eval_to_def:
@@ -168,11 +183,23 @@ Definition eval_to_def:
   eval_to k env (Force x) =
     (do
        v <- eval_to k env x;
-       (wx, binds) <- dest_anyThunk v;
-       case wx of
-         INL v => return v
-       | INR (env, y) => if k = 0 then fail Diverge else
-                           eval_to (k - 1) (subst_funs binds env) y
+       case dest_Tick v of
+         SOME w =>
+           if k = 0 then fail Diverge else
+             eval_to (k - 1) (env ++ [(dummy,w)]) (Force (Var dummy))
+       | NONE =>
+           do (wx, binds) <- dest_anyThunk v;
+              case wx of
+                INL v => return v
+              | INR (env, y) =>
+                  if k = 0 then fail Diverge else
+                    eval_to (k - 1) (subst_funs binds env) y
+           od
+     od) ∧
+  eval_to k env (MkTick x) =
+    (do
+       v <- eval_to k env x;
+       return (DoTick v)
      od) ∧
   eval_to k env (Prim op xs) =
     (case op of
@@ -276,13 +303,26 @@ Proof
     rw [eval_to_def]
     \\ Cases_on ‘eval_to k env x’ \\ fs [])
   >- ((* Force *)
-    rw [eval_to_def]
+    rw []
+    \\ gs [Once eval_to_def]
+    \\ simp [SimpLHS, Once eval_to_def]
+    \\ simp [SimpRHS, Once eval_to_def]
     \\ Cases_on ‘eval_to k env x’ \\ fs []
-    \\ Cases_on ‘dest_anyThunk y’ \\ fs []
-    \\ pairarg_tac \\ gvs []
-    \\ CASE_TAC \\ fs []
-    \\ CASE_TAC \\ fs []
-    \\ IF_CASES_TAC \\ fs [])
+    \\ BasicProvers.TOP_CASE_TAC \\ gs []
+    >- (
+      Cases_on ‘dest_anyThunk y’ \\ gs []
+      \\ pairarg_tac \\ gvs []
+      \\ BasicProvers.TOP_CASE_TAC \\ gs []
+      \\ BasicProvers.TOP_CASE_TAC \\ gs []
+      \\ IF_CASES_TAC \\ gs []
+      \\ first_x_assum irule \\ simp []
+      \\ first_assum (irule_at Any))
+    \\ IF_CASES_TAC \\ gs []
+    \\ first_assum irule \\ simp []
+    \\ first_assum (irule_at Any))
+  >- ((* MkTick *)
+    rw [eval_to_def]
+    \\ Cases_on ‘eval_to k env x’ \\ fs [])
   >- ((* Prim *)
     dsimp []
     \\ strip_tac
